LeanScratch/Fin2.lean
@@ -1,0 +1,10 @@
+import Mathlib.Data.Fin.Fin2
+import Mathlib.Util.WhatsNew
+
+instance Fin2.decEq : DecidableEq (Fin2 n) := fun
+  | .fz, .fs _ | .fs _, .fz => .isFalse Fin2.noConfusion
+  | .fz, .fz => .isTrue rfl
+  | .fs a, .fs b => match decEq a b with
+    | .isTrue p => .isTrue $ p.rec rfl
+    | .isFalse p => .isFalse (p ∘ (Fin2.fs.injEq _ _).mp)
+
