LeanScratch/LogicProof/FirstOrderLogic/Valuation.lean
@@ -10,28 +10,28 @@ structure Interpretation (TA : TNm → Nat) (PA : PNm → Nat) :=
   preds : (nm : PNm) → Vec dom (PA nm) → Prop
 
 -- It does not make sense to talk about a valuation without an Interpretation so we inherit
-structure Valuation (TA : TNm → Nat) (PA : PNm → Nat) extends Interpretation TA PA :=
-  vm : Nat → dom
+structure Valuation (Vars : Nat) (TA : TNm → Nat) (PA : PNm → Nat) extends Interpretation TA PA :=
+  vm : Fin2 Vars → dom
 
-def Valuation.eval (v : Valuation TA PA) : Term TA → v.dom
+def Valuation.eval (v : Valuation Vars TA PA) : Term Vars TA → v.dom
   | .var var => v.vm var
   | .const nm args =>
       v.funcs nm (mapper args)
     where
-      mapper {n} : Vec (Term TA) n → Vec v.dom n
+      mapper {n} : Vec _ n → Vec v.dom n
         | .nil => .nil
         | hd %:: tl => v.eval hd %:: mapper tl
 
-def Valuation.replace (v : Valuation TA PA) (n : Nat) (val : v.dom) : Valuation TA PA :=
+def Valuation.replace (v : Valuation Vars TA PA) (n : Fin2 Vars) (val : v.dom) : Valuation Vars TA PA :=
   { v with vm := fun n' => (if n' = n then val else v.vm n') }
 
-def Valuation.insert (v : Valuation TA PA) (val : v.dom) : Valuation TA PA :=
-  { v with vm := fun | 0 => val | n+1 => v.vm n }
+def Valuation.insert (v : Valuation Vars TA PA) (val : v.dom) : Valuation (Vars.succ) TA PA :=
+  { v with vm := fun | .fz => val | .fs n => v.vm n }
 
 
 -- Definition 7, This is in the text such a joke as they define the logic in a
 -- higher logic. To continue this i will rename the function to what it is.
-def Formula.denote (v : Valuation TA PA) : Formula TA PA → Prop
+def Formula.denote (v : Valuation Vars TA PA) : Formula Vars TA PA → Prop
   -- The additional definition of equality is an unnecacarry addition and should
   -- be ensured by the user
   | .pred p args => v.preds p $ args.map v.eval
@@ -44,9 +44,8 @@ def Formula.denote (v : Valuation TA PA) : Formula TA PA → Prop
   | .iff a b => a.denote v ↔ b.denote v
   | .imp a b => a.denote v → b.denote v
 
-  | .exis b => ∃ x, b.denote $ v.insert x
-  | .univ b => ∀ x, b.denote $ v.insert x
+  | .exis b => ∃ x, (b x).denote v
+  | .univ b => ∀ x, (b x).denote v
 
-def Formula.denote_indep (v : Interpretation TA PA) (form : Formula TA PA) : Prop :=
+def Formula.denote_indep (v : Interpretation TA PA) (form : Formula Vars TA PA) : Prop :=
   ∀ vm, form.denote ⟨v, vm⟩
-
